Uppaal_Networks/UPPAAL_Asm_AbsInt_Refine.thy
@@ -6,8 +6,12 @@ begin
 
 datatype 'a rbt_state_map = RBT_SM "(addr * 'a) rbt"
 
-definition RBT_SM :: "(addr * 'a) rbt \<Rightarrow> 'a state_map" where
-  "RBT_SM tree = SM (Lookup2.lookup tree)"
+fun def :: "'a \<Rightarrow> 'a option \<Rightarrow> 'a" where
+  "def _ (Some v) = v" |
+  "def d _ = d"
+
+definition RBT_SM :: "(addr * 'a) rbt \<Rightarrow> ('a::bot) state_map" where
+  "RBT_SM tree = SM (\<lambda>pc. def \<bottom> (Lookup2.lookup tree pc))"
 
 code_datatype RBT_SM
 
@@ -15,7 +19,7 @@ lemma deepen_RBT_SM[code]:
   "deepen (set states) = propagate (RBT_SM empty) (set states)" sorry
 
 lemma lookup_RBT_SM[code]:
-  "lookup (RBT_SM tree) = Lookup2.lookup tree" sorry
+  "lookup (RBT_SM tree) pc = def \<bottom> (Lookup2.lookup tree pc)" sorry
 
 lemma domain_RBT_SM[code]:
   "domain (RBT_SM tree) = fst ` set (inorder tree)" sorry
@@ -30,7 +34,10 @@ lemma propagate_RBT_SM[code]:
       in upd pc newsts tree
     ) ss oldtree)" sorry
 
+find_consts "('a \<Rightarrow> bool) \<Rightarrow> 'a list \<Rightarrow> bool"
+
 lemma[code]: "step_all op pc (set instates) =
-  Option.these (set (map (\<lambda>ins. step op (pc, ins)) instates))" using in_these_eq by fastforce
+  (Option.these (set (map (\<lambda>ins. step op (pc, ins)) instates)),
+  if list_ex (\<lambda>ins. step op (pc, ins) = None) instates then {StepFailed pc} else {})" sorry
 
 end
